template-coq/theories/Ast.v
@@ -182,9 +182,8 @@ Module TemplateTerm <: Term.
 
   Definition mkApps := mkApps.
 
-  Definition elim_pattern (nsymb npat : nat) := unit.
-  Definition mkPElims (t : term) nsymb npat (l : list (elim_pattern nsymb npat)) :=
-    tRel 0.
+  Definition elim_pattern := unit.
+  Definition mkPElims (n : nat) (t : term) (l : list elim_pattern) := tRel 0.
 
 End TemplateTerm.
 
