template-coq/theories/Environment.v
@@ -21,10 +21,8 @@ Module Type Term.
 
   Parameter (mkApps : term -> list term -> term).
 
-  Parameter (elim_pattern : nat -> nat -> Type).
-  Parameter (mkPElims :
-    term -> forall {nsymb npat}, list (elim_pattern nsymb npat) -> term
-  ).
+  Parameter (elim_pattern : Type).
+  Parameter (mkPElims : nat -> term -> list (elim_pattern) -> term).
 
 End Term.
 
@@ -90,25 +88,20 @@ Module Environment (T : Term).
 
   (** REWRITE RULES *)
 
-  Record rewrite_rule nsymb := mkrew {
+  Record rewrite_rule := mkrew {
     pat_context : context ;
     head : nat ; (* Head symbol, local reference in the block *)
-    elims : list (elim_pattern nsymb #|pat_context|) ;
+    elims : list elim_pattern ;
     rhs : term
   }.
-
-  Arguments pat_context {_} _.
-  Arguments head {_} _.
-  Arguments elims {_} _.
-  Arguments rhs {_} _.
 
   Record rewrite_decl := {
     symbols : list term ; (* Types of the different symbols in the block,
                              can be thought of as a context.
                              The head can depend on the tail.
                            *)
-    rules : list (rewrite_rule #|map (vass nAnon) symbols|) ; (* The actual rewrite rules *)
-    prules : list (rewrite_rule #|map (vass nAnon) symbols|) ;
+    rules : list rewrite_rule ; (* The actual rewrite rules *)
+    prules : list rewrite_rule ;
               (** Parallel rewrite rules to complete the others.
                   They aren't used in the theory itself, only as an intermediary
                   for confluence.
@@ -116,8 +109,9 @@ Module Environment (T : Term).
     rew_universes : universes_decl
   }.
 
-  Definition lhs {nsymb} (r : rewrite_rule nsymb) : term :=
-    mkPElims (tRel (#|r.(pat_context)| + r.(head))) r.(elims).
+  Definition lhs (r : rewrite_rule) : term :=
+    mkPElims
+      #|r.(pat_context)| (tRel (#|r.(pat_context)| + r.(head))) r.(elims).
 
   Inductive global_decl :=
   | ConstantDecl : constant_body -> global_decl
